% Equation 1
\begin{dmath}
{q}=1+\frac{{psi}\, \left({i}-{delta}\, {k}\right)}{{k}}
\end{dmath}
% Equation 2
\begin{dmath}
{q}={sdf}\, \left({theta}\, {z}\, {k}^{{theta}-1}+\frac{{psi}\, \left({i}^{2}-{delta}^{2}\, {k}^{2}\right)}{2\, {k}^{2}}+{q}\, \left(1-{delta}\right)\right)
\end{dmath}
% Equation 3
\begin{dmath}
{k}={i}+{k}\, \left(1-{delta}\right)
\end{dmath}
% Equation 4
\begin{dmath}
{z}={z}\, {rho}+1-{rho}+{eps\_z}
\end{dmath}
% Equation 5
\begin{dmath}
{sdf}=\frac{1}{1+{r}}
\end{dmath}
% Equation 6
\begin{dmath}
{c}={z}\, {k}^{{theta}}-\frac{{psi}\, \left({i}-{delta}\, {k}\right)^{2}}{2\, {k}}-{i}
\end{dmath}
