% Equation 1
\begin{dmath}
{q}_{t}=1+\frac{{psi}\, \left({i}_{t}-{delta}\, {k}_{t-1}\right)}{{k}_{t-1}}
\end{dmath}
% Equation 2
\begin{dmath}
{q}_{t}={sdf}_{t+1}\, \left({theta}\, {z}_{t+1}\, {k}_{t}^{{theta}-1}+\frac{{psi}\, \left({i}_{t+1}^{2}-{delta}^{2}\, {k}_{t}^{2}\right)}{2\, {k}_{t}^{2}}+{q}_{t+1}\, \left(1-{delta}\right)\right)
\end{dmath}
% Equation 3
\begin{dmath}
{k}_{t}={i}_{t}+{k}_{t-1}\, \left(1-{delta}\right)
\end{dmath}
% Equation 4
\begin{dmath}
{z}_{t}={rho}\, {z}_{t-1}+1-{rho}+{eps\_z}_{t}
\end{dmath}
% Equation 5
\begin{dmath}
{sdf}_{t}=\frac{1}{1+{r}}\, \left(\frac{{c}_{t}}{{c}_{t-1}}\right)^{\left(-{gamma}\right)}
\end{dmath}
% Equation 6
\begin{dmath}
{c}_{t}={z}_{t}\, {k}_{t-1}^{{theta}}-\frac{{psi}\, \left({i}_{t}-{delta}\, {k}_{t-1}\right)^{2}}{2\, {k}_{t-1}}-{i}_{t}
\end{dmath}
