% Equation 1
\begin{dmath}
{q}_{t}=1
\end{dmath}
% Equation 2
\begin{dmath}
1={sdf}_{t+1}\, \left({theta}\, {z}_{t+1}\, {k}_{t}^{{theta}-1}+1-{delta}\right)
\end{dmath}
% Equation 3
\begin{dmath}
{k}_{t}={i}_{t}+\left(1-{delta}\right)\, {k}_{t-1}
\end{dmath}
% Equation 4
\begin{dmath}
{z}_{t}={rho}\, {z}_{t-1}+1-{rho}+{eps\_z}_{t}
\end{dmath}
% Equation 5
\begin{dmath}
{sdf}_{t}=\frac{1}{1+{r}}\, \left(\frac{{c}_{t}}{{c}_{t-1}}\right)^{\left(-{gamma}\right)}
\end{dmath}
% Equation 6
\begin{dmath}
{c}_{t}={z}_{t}\, {k}_{t-1}^{{theta}}-{i}_{t}
\end{dmath}
